Add the next-generation implementation’s documentation

src/Equivalence_Reasoner.thy
@@ -1,14 +1,41 @@
+section \<open>Implementation\<close>
+
 theory Equivalence_Reasoner
 imports
   Main
   "HOL-Eisbach.Eisbach_Tools"
+    \<comment>\<open>Besides Eisbach, we use the @{attribute uncurry} attribute from the Eisbach tools.\<close>
 begin
+
+text \<open>
+  We start with defining what an equivalence class, a representative, and a canonical form are.
+\<close>
 
 definition equivalence_class :: "'a \<Rightarrow> ('a \<Rightarrow> 'a \<Rightarrow> bool) \<Rightarrow> 'a set" (\<open>[_]\<^bsub>_\<^esub>\<close>) where
   "[x]\<^bsub>R\<^esub> = {y. R x y}"
 
-definition frozen_equivalence_class :: "'a \<Rightarrow> ('a \<Rightarrow> 'a \<Rightarrow> bool) \<Rightarrow> 'a set" where
-  "frozen_equivalence_class = equivalence_class"
+definition representative :: "'a set \<Rightarrow> 'a" where
+  "representative X = (SOME x. x \<in> X)"
+
+abbreviation canonical :: "('a \<Rightarrow> 'a \<Rightarrow> bool) \<Rightarrow> 'a \<Rightarrow> 'a" where
+  "canonical R x \<equiv> representative [x]\<^bsub>R\<^esub>"
+
+text \<open>
+  The key idea of our implementation is to turn equivalences into equalities of equivalence classes
+  and solve the resulting goals using the Simplifier. The translation from equivalences to
+  equalities that are ready for simplification works as follows:
+
+    \<^item> First, each equivalence \<^term>\<open>R x y\<close> is turned into \<^term>\<open>[x]\<^bsub>R\<^esub> = [y]\<^bsub>R\<^esub>\<close>.
+
+    \<^item> Second, each equivalence class construction \<^term>\<open>[x]\<^bsub>R\<^esub>\<close> for which there is a compatibility
+      rule \<^term>\<open>R x y\<close> is turned into \<^term>\<open>[y]\<^bsub>R\<^esub>\<close>. This is done repeatedly until no such
+      replacement is possible anymore.
+
+  Both of these steps involve converting equivalences into equalities of equivalence classes: the
+  first step converts subterms of the goal, the second step converts compatibility rules, generating
+  rewrite rules that perform the described replacement. We prove a lemma that enables such
+  conversions.
+\<close>
 
 lemma equivalence_is_equivalence_class_equality:
   assumes "equivp R"
@@ -17,53 +44,138 @@ lemma equivalence_is_equivalence_class_equality:
   unfolding equivp_def and equivalence_class_def
   by auto
 
+text \<open>
+  Actually, performing the second of the above steps will typically result in endless looping. To
+  see why, consider the compatibility rule \<^term>\<open>\<And>x. R (f x) (f (canonical R x))\<close>, which is
+  probably one of the simplest of its kind. Let us assume the first of the above steps has produced
+  a subterm \<^term>\<open>[f (f x)]\<^bsub>R\<^esub>\<close>. We want the second step to turn this subterm first into
+  \<^term>\<open>[f (canonical R (f x))]\<^bsub>R\<^esub>\<close> and further into \<^term>\<open>[f (canonical R (f (canonical R x)))]\<^bsub>R\<^esub>\<close>.
+  These translations are surely possible (the second one uses the fact that \<^term>\<open>canonical R (f x)\<close>
+  is shorthand for \<^term>\<open>representative [f x]\<^bsub>R\<^esub>\<close> and thus contains another equivalence class
+  construction). However, they are not the only ones that can be performed, as the compatibility
+  rule permits the replacement of any subterm of the form \<open>[f _]\<^bsub>R\<^esub>\<close> by another subterm of this
+  form, making it possible to perform further such replacements \<^emph>\<open>ad infinitum\<close>.
+
+  We solve this problem by letting the replacement subterms use an alternative equivalence class
+  constructor \<^term>\<open>frozen_equivalence_class\<close> instead of the standard one. The constant
+  \<^term>\<open>frozen_equivalence_class\<close> equals \<^const>\<open>equivalence_class\<close>, but its use makes rewrite rules
+  that require \<^const>\<open>equivalence_class\<close> unapplicable. With this correction in place, the second
+  step turns \<^term>\<open>[f (f x)]\<^bsub>R\<^esub>\<close> into \<^term>\<open>frozen_equivalence_class (f (canonical R (f x))) R\<close> and
+  this further into
+  \<^term>\<open>frozen_equivalence_class (f (representative (frozen_equivalence_class (f (canonical R x)) R))) R\<close>.
+  From there, no further translations are possible.
+\<close>
+
+definition frozen_equivalence_class :: "'a \<Rightarrow> ('a \<Rightarrow> 'a \<Rightarrow> bool) \<Rightarrow> 'a set" where
+  "frozen_equivalence_class = equivalence_class"
+
 lemma equivalence_is_right_frozen_equivalence_class_equality:
   assumes "equivp R"
   shows "R x y \<longleftrightarrow> [x]\<^bsub>R\<^esub> = frozen_equivalence_class y R"
   unfolding frozen_equivalence_class_def
   using equivalence_is_equivalence_class_equality [OF assms] .
 
-definition representative :: "'a set \<Rightarrow> 'a" where
-  "representative X = (SOME x. x \<in> X)"
+text \<open>
+  We introduce a helper method \<^theory_text>\<open>generate_relax_inclusions\<close> that takes a set of inclusions and a
+  relation~\<^term>\<open>R\<close> and computes the set of all inclusions that can be derived from the inclusions
+  in the given set using only reflexivity and transitivity and furthermore have the form \<open>_ \<le> R\<close>.
+  The inclusions in the resulting set are called relax inclusions, since they are supposed to be fed
+  into the \<^theory_text>\<open>relax\<close> method defined below.
 
-abbreviation canonical :: "('a \<Rightarrow> 'a \<Rightarrow> bool) \<Rightarrow> 'a \<Rightarrow> 'a" where
-  "canonical R x \<equiv> representative [x]\<^bsub>R\<^esub>"
+  The \<^theory_text>\<open>generate_relax_inclusions\<close> method does not receive its input inclusions via a fact argument,
+  but as goal premises. This is because it needs to iterate over them, and the only possible way to
+  do that in Eisbach seems to involve removing them one by one, which in turn seems to be possible
+  only if storing them as premises (premises can be removed via the @{attribute thin} attribute).
+
+  The \<^theory_text>\<open>generate_relax_inclusions\<close> method considers only those premises that are of the shape
+  \<^term>\<open>S \<le> T\<close> where \<^term>\<open>S\<close>~and~\<^term>\<open>T\<close> have the same type as~\<^term>\<open>R\<close>. It drops all other
+  premises.
+
+  Output inclusions are delivered as the premises of the resulting goal, since methods can
+  communicate information to their callers only via the goal state.
+
+  To iterate through the input inclusions, the \<^theory_text>\<open>generate_relax_inclusions\<close> method recursively
+  invokes itself. Since it already uses the goal premises for storing the shrinking set of input
+  inclusions, it stores the growing set of output inclusions in a fact argument \<^theory_text>\<open>accumulator\<close>,
+  which is amended at each recursive invocation. Users of the method should not specify this
+  argument, so that the method starts with \<^theory_text>\<open>accumulator\<close> being the empty fact list.
+\<close>
 
 method generate_relax_inclusions for R :: "'a \<Rightarrow> 'a \<Rightarrow> bool" uses accumulator = (
+  \<comment> \<open>Pick an input inclusion of the form \<open>_ \<le> R\<close>, called a base inclusion, and process it:\<close>
   match premises in base [thin]: "S \<le> R" (cut) for S \<Rightarrow> \<open>
+    \<comment> \<open>If the base inclusion is extendable, add its extensions to the set of input inclusions:\<close>
     (
+      \<comment> \<open>Add the extensions of the base inclusion to the set of input inclusions:\<close>
       match premises in extensions [thin]: "_ \<le> S" (multi, cut) \<Rightarrow> \<open>
         insert extensions [THEN order_trans, OF base]
       \<close>
     )?,
+    \<comment> \<open>Continue with the base inclusion added to the set of output inclusions:\<close>
     generate_relax_inclusions R accumulator: accumulator base
   \<close> |
+  \<comment> \<open>Remove all unused input inclusions and invalid premises:\<close>
   (match premises in leftover [thin]: _ (multi, cut) \<Rightarrow> \<open>succeed\<close>)?,
+  \<comment> \<open>Add \<^term>\<open>R \<le> R\<close> to the set of output inclusions and return the result:\<close>
   insert accumulator order_refl [of R]
 )
 
+text \<open>
+  We introduce a helper method \<^theory_text>\<open>relax\<close> that takes a set of inclusions and turns all goal premises
+  of the shape \<open>P\<^sub>1 \<Longrightarrow> \<cdots> \<Longrightarrow> P\<^sub>n \<Longrightarrow> S x y\<close> for which \<^term>\<open>S \<le> R\<close> is among the given conclusions
+  into \<open>P\<^sub>1 \<Longrightarrow> \<cdots> \<Longrightarrow> P\<^sub>n \<Longrightarrow> R x y\<close>, while dropping all other premises.
+
+  The \<^theory_text>\<open>relax\<close> method recursively invokes itself. It removes the input premises one by one from the
+  goal and collects the output premises in a fact argument \<^theory_text>\<open>accumulator\<close>. As with
+  @{method generate_relax_inclusions}, users of \<^theory_text>\<open>relax\<close> should not specify the \<^theory_text>\<open>accumulator\<close>
+  argument, so that the method starts with \<^theory_text>\<open>accumulator\<close> being the empty fact list.
+\<close>
+
 method relax uses inclusions accumulator = (
+  \<comment> \<open>Pick a premise and process it:\<close>
   match premises in premise [thin]: _ (cut) \<Rightarrow> \<open>
+    \<comment> \<open>Get the inclusion that fits the premise and process the premise using it:\<close>
     match inclusions in inclusion: "S \<le> _" for S :: "'a \<Rightarrow> 'a \<Rightarrow> bool" \<Rightarrow> \<open>
+      \<comment> \<open>Make sure the inclusion fits the premise (if it does not, backtrack):\<close>
       match premise [uncurry] in
         "S _ _" (cut) \<Rightarrow> \<open>succeed\<close> \<bar>
         "_ \<Longrightarrow> S _ _" (cut) \<Rightarrow> \<open>succeed\<close>,
+      \<comment> \<open>Continue with the relaxed premise added to the set of output premises:\<close>
       relax
         inclusions: inclusions
         accumulator: accumulator premise [THEN inclusion [THEN predicate2D]]
     \<close> |
+    \<comment> \<open>Continue with the set of output premises unchanged:\<close>
     relax
       inclusions: inclusions
       accumulator: accumulator
   \<close> |
+  \<comment> \<open>Return the set of output premises:\<close>
   insert accumulator
 )
 
+text \<open>
+  We introduce a helper method \<^theory_text>\<open>raw_equivalence\<close> that essentially works like \<^theory_text>\<open>try_equivalence\<close>.
+  The only difference is that \<^theory_text>\<open>raw_equivalence\<close> does not use the named theorems \<^theory_text>\<open>equivalence\<close>,
+  \<^theory_text>\<open>inclusion\<close>, and \<^theory_text>\<open>compatibility\<close>, but receives the respective fact lists as fact arguments. This
+  enables us to use \<^theory_text>\<open>raw_equivalence\<close> in the implementation of the \<^theory_text>\<open>equivalence\<close> method. If
+  \<^theory_text>\<open>equivalence\<close> would invoke \<^theory_text>\<open>try_equivalence\<close> instead of \<^theory_text>\<open>raw_equivalence\<close>, the facts that come
+  from the unaugmented named theorems \<^theory_text>\<open>equivalence\<close>, \<^theory_text>\<open>inclusion\<close>, and \<^theory_text>\<open>compatibility\<close> would be
+  duplicated: \<^theory_text>\<open>equivalence\<close> would augment all named theorems with the corresponding declaration
+  arguments and could only use the resulting fact lists in its invocation of \<^theory_text>\<open>try_equivalence\<close>,
+  which would augment the named theorems with these fact lists.
+\<close>
+
 method raw_equivalence uses equivalence inclusion compatibility simplification = (
+  \<comment> \<open>Turn all chained facts into goal premises and try to solve the resulting goal:\<close>
   -, use nothing in \<open>
+    \<comment> \<open>Get the equivalence relation that is used by the conclusion and perform relaxation using it:\<close>
     match equivalence in current_equivalence: "equivp R" for R \<Rightarrow> \<open>
+      \<comment> \<open>Make sure the equivalence relation is used by the conclusion (if it is not, backtrack):\<close>
       match conclusion in "R _ _"  (cut) \<Rightarrow> \<open>succeed\<close>,
+      \<comment> \<open>If any premises exist, relax all premises that can be relaxed and drop all others:\<close>
       (
+        \<comment> \<open>Relax all premises that can be relaxed and drop all others:\<close>
         match premises in original_premises [thin]: _ (multi, cut) \<Rightarrow> \<open>
           insert inclusion,
           generate_relax_inclusions R,
@@ -74,19 +186,31 @@ method raw_equivalence uses equivalence inclusion compatibility simplification =
         \<close>
       )?
     \<close>,
+    \<comment> \<open>Turn equivalences into equalities, taking compatibility rules into account:\<close>
     simp (no_asm_use) only:
       equivalence
         [THEN equivalence_is_equivalence_class_equality]
       compatibility
         [simplified equivalence [THEN equivalence_is_right_frozen_equivalence_class_equality]],
+    \<comment> \<open>Unfreeze all frozen equivalence class constructions:\<close>
     (unfold frozen_equivalence_class_def)?,
+    \<comment> \<open>Simplify the conclusion, using the premises and the given simplification rules:\<close>
     (simp (no_asm_simp) only: simplification)?
   \<close>
 )
 
+text \<open>
+  We declare the named theorems \<^theory_text>\<open>equivalence\<close>, \<^theory_text>\<open>inclusion\<close>, and \<^theory_text>\<open>compatibility\<close>.
+\<close>
+
 named_theorems equivalence and inclusion and compatibility
 
+text \<open>
+  Finally, we implement the methods we offer to the user.
+\<close>
+
 method try_equivalence uses simplification declares equivalence inclusion compatibility = (
+  \<comment> \<open>Invoke @{method raw_equivalence} with the augmented named theorems and the simplification rules:\<close>
   raw_equivalence
     equivalence: equivalence
     inclusion: inclusion
@@ -95,12 +219,18 @@ method try_equivalence uses simplification declares equivalence inclusion compat
 )
 
 method equivalence uses simplification declares equivalence inclusion compatibility = (
+  \<comment> \<open>Invoke @{method raw_equivalence} with the augmented named theorems and the simplification rules:\<close>
   raw_equivalence
     equivalence: equivalence
     inclusion: inclusion
     compatibility: compatibility
     simplification: simplification;
+  \<comment> \<open>Fail (only done if @{method raw_equivalence} left a goal, because of the \<^theory_text>\<open>;\<close>-combinator):\<close>
   fail
 )
+
+text \<open>
+  This concludes the implementation of the equivalence reasoner.
+\<close>
 
 end
